James C - partially finished chapter 13

isabelle/Chapter13_1_Types.thy
@@ -10,8 +10,6 @@ datatype type =
 | Prod type type
 | Void
 | Sum type type
-| Ind type
-| Coind type
 
 primrec is_valid :: "unit env => type => bool"
 where "is_valid del (TyVar v) = v in del"
@@ -21,8 +19,15 @@ where "is_valid del (TyVar v) = v in del"
     | "is_valid del (Prod t1 t2) = (is_valid del t1 & is_valid del t2)"
     | "is_valid del Void = True"
     | "is_valid del (Sum t1 t2) = (is_valid del t1 & is_valid del t2)"
-    | "is_valid del (Ind t) = is_valid (extend del ()) t"
-    | "is_valid del (Coind t) = is_valid (extend del ()) t"
+
+primrec is_positive :: "var => type => bool"
+where "is_positive t (TyVar v) = (v = t)"
+    | "is_positive t Nat = True"
+    | "is_positive t (Arrow t1 t2) = (is_valid empty_env t1 & is_positive t t2)"
+    | "is_positive t Unit = True"
+    | "is_positive t (Prod t1 t2) = (is_positive t t1 & is_positive t t2)"
+    | "is_positive t Void = True"
+    | "is_positive t (Sum t1 t2) = (is_positive t t1 & is_positive t t2)"
 
 primrec type_insert :: "var => type => type"
 where "type_insert n (TyVar v) = TyVar (incr n v)"
@@ -32,8 +37,6 @@ where "type_insert n (TyVar v) = TyVar (incr n v)"
     | "type_insert n (Prod e1 e2) = Prod (type_insert n e1) (type_insert n e2)"
     | "type_insert n Void = Void"
     | "type_insert n (Sum e1 e2) = Sum (type_insert n e1) (type_insert n e2)"
-    | "type_insert n (Ind t) = Ind (type_insert (next n) t)"
-    | "type_insert n (Coind t) = Coind (type_insert (next n) t)"
 
 primrec type_remove :: "var => type => type"
 where "type_remove n (TyVar v) = TyVar (subr n v)"
@@ -43,8 +46,6 @@ where "type_remove n (TyVar v) = TyVar (subr n v)"
     | "type_remove n (Prod e1 e2) = Prod (type_remove n e1) (type_remove n e2)"
     | "type_remove n Void = Void"
     | "type_remove n (Sum e1 e2) = Sum (type_remove n e1) (type_remove n e2)"
-    | "type_remove n (Ind t) = Ind (type_remove (next n) t)"
-    | "type_remove n (Coind t) = Coind (type_remove (next n) t)"
 
 primrec type_subst' :: "var => type => type => type"
 where "type_subst' n e' (TyVar v) = (if v = n then e' else TyVar v)"
@@ -54,8 +55,6 @@ where "type_subst' n e' (TyVar v) = (if v = n then e' else TyVar v)"
     | "type_subst' n e' (Prod e1 e2) = Prod (type_subst' n e' e1) (type_subst' n e' e2)"
     | "type_subst' n e' Void = Void"
     | "type_subst' n e' (Sum e1 e2) = Sum (type_subst' n e' e1) (type_subst' n e' e2)"
-    | "type_subst' n e' (Ind t) = Ind (type_subst' (next n) (type_insert first e') t)"
-    | "type_subst' n e' (Coind t) = Coind (type_subst' (next n) (type_insert first e') t)"
 
 definition type_subst :: "type => type => type"
 where "type_subst e' e = type_remove first (type_subst' first (type_insert first e') e)"
@@ -63,8 +62,7 @@ where "type_subst e' e = type_remove first (type_subst' first (type_insert first
 lemma [simp]: "type_remove n (type_insert n e) = e"
 by (induction e arbitrary: n, simp_all)
 
-lemma [simp]: "canswap m n ==> 
-        type_insert m (type_insert n e) = type_insert (next n) (type_insert m e)"
+lemma [simp]: "canswap m n ==> type_insert m (type_insert n e) = type_insert (next n) (type_insert m e)"
 by (induction e arbitrary: n m, simp_all)
 
 end
